Source/DafnyCompilers/Values.dfy
@@ -7,6 +7,8 @@ module Values {
   import DafnyCompilerCommon.AST.Exprs
   import DafnyCompilerCommon.AST.Types
 
+  type Context = map<string, Value>
+
   datatype Value =
     | Bool(b: bool)
     | Char(c: char)
@@ -18,7 +20,7 @@ module Values {
     | Multiset(ms: multiset<Value>)
     | Seq(sq: seq<Value>)
     | Set(st: set<Value>)
-    | Abs(vars: seq<string>, body: Exprs.T)
+    | Closure(ctx: Context, vars: seq<string>, body: Exprs.T)
   {
     predicate method HasType(ty: Types.T) {
       match (this, ty) // FIXME tests on other side
@@ -37,7 +39,7 @@ module Values {
           forall x | x in sq :: x.HasType(eT)
         case (Set(st), Collection(true, Set, eT)) =>
           forall x | x in st :: x.HasType(eT)
-        case (Abs(vars, body), Function(args, ret)) =>
+        case (Closure(ctx, vars, body), Function(args, ret)) =>
           true // FIXME: Need a typing relation on terms, not just values
 
         // DISCUSS: Better way to write this?  Need exhaustivity checking
@@ -51,7 +53,7 @@ module Values {
         case (Multiset(ms), _) => false
         case (Seq(sq), _) => false
         case (Set(st), _) => false
-        case (Abs(vars, body), _) => false
+        case (Closure(ctx, vars, body), _) => false
     }
 
     function method Cast(ty: Types.T) : (v: Option<Value>)
